translator/repl/ml_repl_stepScript.sml
@@ -11,16 +11,19 @@ open BytecodeTheory mmlParseTheory mmlPEGTheory;
 open arithmeticTheory listTheory finite_mapTheory pred_setTheory;
 open ml_translatorLib ml_translatorTheory std_preludeTheory;
 
-val _ = translation_extends "std_prelude";
 
 (* translator setup *)
+
+val _ = translation_extends "std_prelude";
 
 val _ = add_preferred_thy "termination";
 val _ = add_preferred_thy "compilerTermination";
 
-val lemma = prove(
+val NOT_NIL_AND_LEMMA = prove(
   ``(b <> [] /\ x) = if b = [] then F else x``,
   Cases_on `b` THEN FULL_SIMP_TAC std_ss []);
+
+val extra_preprocessing = ref [MEMBER_INTRO,MAP];
 
 fun def_of_const tm = let
   val res = dest_thy_const tm handle HOL_ERR _ =>
@@ -35,12 +38,14 @@ fun def_of_const tm = let
             def_from_thy "compilerTermination" name handle HOL_ERR _ =>
             def_from_thy (#Thy res) name handle HOL_ERR _ =>
             failwith ("Unable to find definition of " ^ name)
-  val def = def |> RW [MEMBER_INTRO,MAP]
+  val def = def |> RW (!extra_preprocessing)
                 |> CONV_RULE (DEPTH_CONV BETA_CONV)
-                |> SIMP_RULE bool_ss [IN_INSERT,NOT_IN_EMPTY] |> RW [lemma]
+                |> SIMP_RULE bool_ss [IN_INSERT,NOT_IN_EMPTY]
+                |> RW [NOT_NIL_AND_LEMMA]
   in def end
 
 val _ = (find_def_for_const := def_of_const);
+
 
 (* compiler *)
 
@@ -51,9 +56,11 @@ val fapply_thm = prove(
 val _ = translate fapply_thm;
 val _ = translate compile_top_def;
 
+
 (* elaborator *)
 
 val _ = translate (def_of_const ``elab_top``);
+
 
 (* parsing: peg_exec and mmlPEG *)
 
@@ -72,6 +79,7 @@ val _ = translate (def_of_const ``coreloop`` |> RW [INTRO_FLOOKUP]
                    |> SPEC_ALL |> RW1 [FUN_EQ_THM]);
 val _ = translate (def_of_const ``peg_exec``);
 
+
 (* parsing: mmlvalid *)
 
 val LENGTH_LEMMA = prove(
@@ -88,7 +96,7 @@ val monad_unitbind_assert = prove(
   Cases THEN EVAL_TAC THEN SIMP_TAC std_ss []);
 
 val _ = translate (mmlvalidTheory.mml_okrule_eval_th
-                   |> RW [monad_unitbind_assert,lemma,if_and_lemma])
+          |> RW [monad_unitbind_assert,NOT_NIL_AND_LEMMA,if_and_lemma])
 
 val mml_okrule_side_def = prove(
   ``!x y. mml_okrule_side x y = T``,
@@ -104,11 +112,19 @@ val res = translate
     (mmlvalidTheory.mmlvalidL_def |> CONJUNCTS))
    |> map GEN_ALL |> LIST_CONJ)
 
+
 (* parsing: ptree converstion *)
 
-val _ = translate (def_of_const ``ptree_Type``); (* uses cheat *)
-val _ = translate (def_of_const ``ptree_Expr``); (* uses cheat *)
+val OPTION_BIND_THM = prove(
+  ``!x y. OPTION_BIND x y = case x of NONE => NONE | SOME i => y i``,
+  Cases THEN SRW_TAC [] []);
+
+val _ = (extra_preprocessing :=
+  [MEMBER_INTRO,MAP,OPTION_BIND_THM,monad_unitbind_assert]);
+
+val _ = translate (def_of_const ``ptree_Expr``);
 val _ = translate (def_of_const ``ptree_REPLTop``);
+
 
 (* parsing: top-level parser *)
 
@@ -123,5 +139,6 @@ val parse_top_side_def = prove(
   THEN FULL_SIMP_TAC std_ss [INTRO_FLOOKUP] THEN POP_ASSUM MP_TAC
   THEN CONV_TAC (DEPTH_CONV ETA_CONV) THEN FULL_SIMP_TAC std_ss [])
   |> update_precondition;
+
 
 val _ = export_theory();
